specs/L2InteropCommitmentTree/L2InteropCommitmentTree/Common/switch_2003501192971474853_user.lean
@@ -13,12 +13,13 @@ section
 
 open Clear EVMState Ast Expr Stmt FunctionDefinition State Interpreter ExecLemmas OutOfFuelLemmas Abstraction YulNotation PrimOps ReasoningPrinciple Utilities generated.L2InteropCommitmentTree L2InteropCommitmentTree
 
-def A_switch_2003501192971474853 (s₀ s₉ : State) : Prop := sorry
+def A_switch_2003501192971474853 (s₀ s₉ : State) : Prop := switch_2003501192971474853_concrete_of_code.1 s₀ s₉
 
 lemma switch_2003501192971474853_abs_of_concrete {s₀ s₉ : State} :
   Spec switch_2003501192971474853_concrete_of_code s₀ s₉ →
   Spec A_switch_2003501192971474853 s₀ s₉ := by
-  sorry
+  intro h
+  simpa [A_switch_2003501192971474853] using h
 
 end
 
