specs/L2InteropCommitmentTree/L2InteropCommitmentTree/Common/switch_8961670722464898128_user.lean
@@ -18,12 +18,13 @@ section
 
 open Clear EVMState Ast Expr Stmt FunctionDefinition State Interpreter ExecLemmas OutOfFuelLemmas Abstraction YulNotation PrimOps ReasoningPrinciple Utilities L2InteropCommitmentTree.Common generated.L2InteropCommitmentTree L2InteropCommitmentTree
 
-def A_switch_8961670722464898128 (s₀ s₉ : State) : Prop := sorry
+def A_switch_8961670722464898128 (s₀ s₉ : State) : Prop := switch_8961670722464898128_concrete_of_code.1 s₀ s₉
 
 lemma switch_8961670722464898128_abs_of_concrete {s₀ s₉ : State} :
   Spec switch_8961670722464898128_concrete_of_code s₀ s₉ →
   Spec A_switch_8961670722464898128 s₀ s₉ := by
-  sorry
+  intro h
+  simpa [A_switch_8961670722464898128] using h
 
 end
 
