specs/L2InteropCommitmentTree/L2InteropCommitmentTree/array_dataslot_array_bytes32_dyn_storage_ptr_user.lean
@@ -10,13 +10,13 @@ section
 
 open Clear EVMState Ast Expr Stmt FunctionDefinition State Interpreter ExecLemmas OutOfFuelLemmas Abstraction YulNotation PrimOps ReasoningPrinciple Utilities 
 
-def A_array_dataslot_array_bytes32_dyn_storage_ptr (data : Identifier) (ptr : Literal) (s₀ s₉ : State) : Prop := sorry
+def A_array_dataslot_array_bytes32_dyn_storage_ptr (data : Identifier) (ptr : Literal) (s₀ s₉ : State) : Prop := array_dataslot_array_bytes32_dyn_storage_ptr_concrete_of_code.1 data ptr s₀ s₉
 
 lemma array_dataslot_array_bytes32_dyn_storage_ptr_abs_of_concrete {s₀ s₉ : State} {data ptr} :
   Spec (array_dataslot_array_bytes32_dyn_storage_ptr_concrete_of_code.1 data ptr) s₀ s₉ →
   Spec (A_array_dataslot_array_bytes32_dyn_storage_ptr data ptr) s₀ s₉ := by
-  unfold array_dataslot_array_bytes32_dyn_storage_ptr_concrete_of_code A_array_dataslot_array_bytes32_dyn_storage_ptr
-  sorry
+  intro h
+  simpa [A_array_dataslot_array_bytes32_dyn_storage_ptr] using h
 
 end
 
