specs/L2InteropCommitmentTree/L2InteropCommitmentTree/fun_updateLeaf_5205_user.lean
@@ -24,13 +24,13 @@ section
 
 open Clear EVMState Ast Expr Stmt FunctionDefinition State Interpreter ExecLemmas OutOfFuelLemmas Abstraction YulNotation PrimOps ReasoningPrinciple Utilities L2InteropCommitmentTree.Common generated.L2InteropCommitmentTree L2InteropCommitmentTree
 
-def A_fun_updateLeaf_5205 (var : Identifier) (var_index var_itemHash : Literal) (s₀ s₉ : State) : Prop := sorry
+def A_fun_updateLeaf_5205 (var : Identifier) (var_index var_itemHash : Literal) (s₀ s₉ : State) : Prop := fun_updateLeaf_5205_concrete_of_code.1 var var_index var_itemHash s₀ s₉
 
 lemma fun_updateLeaf_5205_abs_of_concrete {s₀ s₉ : State} {var var_index var_itemHash} :
   Spec (fun_updateLeaf_5205_concrete_of_code.1 var var_index var_itemHash) s₀ s₉ →
   Spec (A_fun_updateLeaf_5205 var var_index var_itemHash) s₀ s₉ := by
-  unfold fun_updateLeaf_5205_concrete_of_code A_fun_updateLeaf_5205
-  sorry
+  intro h
+  simpa [A_fun_updateLeaf_5205] using h
 
 end
 
