specs/L2InteropCommitmentTree/L2InteropCommitmentTree/mapping_index_access_mapping_uint256_struct_IMTLeaf_storage_of_uint256_5199_user.lean
@@ -10,13 +10,13 @@ section
 
 open Clear EVMState Ast Expr Stmt FunctionDefinition State Interpreter ExecLemmas OutOfFuelLemmas Abstraction YulNotation PrimOps ReasoningPrinciple Utilities 
 
-def A_mapping_index_access_mapping_uint256_struct_IMTLeaf_storage_of_uint256_5199 (dataSlot : Identifier) (key : Literal) (s₀ s₉ : State) : Prop := sorry
+def A_mapping_index_access_mapping_uint256_struct_IMTLeaf_storage_of_uint256_5199 (dataSlot : Identifier) (key : Literal) (s₀ s₉ : State) : Prop := mapping_index_access_mapping_uint256_struct_IMTLeaf_storage_of_uint256_5199_concrete_of_code.1 dataSlot key s₀ s₉
 
 lemma mapping_index_access_mapping_uint256_struct_IMTLeaf_storage_of_uint256_5199_abs_of_concrete {s₀ s₉ : State} {dataSlot key} :
   Spec (mapping_index_access_mapping_uint256_struct_IMTLeaf_storage_of_uint256_5199_concrete_of_code.1 dataSlot key) s₀ s₉ →
   Spec (A_mapping_index_access_mapping_uint256_struct_IMTLeaf_storage_of_uint256_5199 dataSlot key) s₀ s₉ := by
-  unfold mapping_index_access_mapping_uint256_struct_IMTLeaf_storage_of_uint256_5199_concrete_of_code A_mapping_index_access_mapping_uint256_struct_IMTLeaf_storage_of_uint256_5199
-  sorry
+  intro h
+  simpa [A_mapping_index_access_mapping_uint256_struct_IMTLeaf_storage_of_uint256_5199] using h
 
 end
 
