specs/L2InteropCommitmentTree/L2InteropCommitmentTree/storage_array_index_access_bytes32_dyn_ptr_5214_user.lean
@@ -12,13 +12,13 @@ section
 
 open Clear EVMState Ast Expr Stmt FunctionDefinition State Interpreter ExecLemmas OutOfFuelLemmas Abstraction YulNotation PrimOps ReasoningPrinciple Utilities L2InteropCommitmentTree.Common generated.L2InteropCommitmentTree L2InteropCommitmentTree
 
-def A_storage_array_index_access_bytes32_dyn_ptr_5214 (slot offset : Identifier) (index : Literal) (s₀ s₉ : State) : Prop := sorry
+def A_storage_array_index_access_bytes32_dyn_ptr_5214 (slot offset : Identifier) (index : Literal) (s₀ s₉ : State) : Prop := storage_array_index_access_bytes32_dyn_ptr_5214_concrete_of_code.1 slot offset index s₀ s₉
 
 lemma storage_array_index_access_bytes32_dyn_ptr_5214_abs_of_concrete {s₀ s₉ : State} {slot offset index} :
   Spec (storage_array_index_access_bytes32_dyn_ptr_5214_concrete_of_code.1 slot offset index) s₀ s₉ →
   Spec (A_storage_array_index_access_bytes32_dyn_ptr_5214 slot offset index) s₀ s₉ := by
-  unfold storage_array_index_access_bytes32_dyn_ptr_5214_concrete_of_code A_storage_array_index_access_bytes32_dyn_ptr_5214
-  sorry
+  intro h
+  simpa [A_storage_array_index_access_bytes32_dyn_ptr_5214] using h
 
 end
 
